Only need concrete arithmetic semantics

Stlc.v
@@ -4,27 +4,59 @@ Require Import Metalib.Metatheory.
 Parameter X : expvar.
 Parameter Y : expvar.
 
-Definition n_to_expr(a: n) := tm_const (const_field a).
+(** Notation on Stlc_Ott *)
+Coercion tm_var_f: expvar >-> exp.
+Coercion const_field: nat >-> constant.
+Coercion tm_constant: constant >-> exp.
 
-Coercion const_field: n >-> Stlc_Ott.const.
-Coercion tm_const: Stlc_Ott.const >-> Stlc_Ott.exp.
-Coercion n_to_expr: n >-> Stlc_Ott.exp.
+Declare Custom Entry stlc_ty.
+Declare Custom Entry stlc.
+Notation "<{ e }>" := e (e custom stlc at level 99).
+Notation "<{{ e }}>" := e (e custom stlc_ty at level 99).
+Notation "( x )" := x (in custom stlc, x at level 99).
+Notation "( x )" := x (in custom stlc_ty, x at level 99).
+Notation "x" := x (in custom stlc at level 0, x constr at level 0).
+Notation "x" := x (in custom stlc_ty at level 0, x constr at level 0).
+Notation "S -> T" := (ty_arrow S T) (in custom stlc_ty at level 50, right associativity).
+Notation "x y" := (tm_app x y) (in custom stlc at level 1, left associativity).
+Notation "\ x : t , y" :=
+  (open_exp_wrt_exp (tm_abs t y) x) (in custom stlc at level 90,
+                     t custom stlc_ty at level 99,
+                     y custom stlc at level 99,
+                     left associativity).
 
-Definition div_compute(a: nat) :=
-  open_exp_wrt_exp (tm_abs ty_field (tm_binop (const_field 100) tm_div (tm_var_f X))) (tm_var_f X).
+Notation "{ x }" := x (in custom stlc at level 1, x constr).
 
-Definition div_check (a w: nat) :=
-  open_exp_wrt_exp (
-      open_exp_wrt_exp (
-          tm_abs ty_field (
-                   open_exp_wrt_exp (
-                       tm_abs ty_field (tm_binop (tm_var_f X) tm_mul (tm_var_f Y)))
-                              (tm_var_f Y)
-                     )
-                 )
-          (tm_var_f Y)
-    ) (tm_var_f X).
+Notation "'Field'" := ty_field (in custom stlc_ty at level 0).
+Notation "'Bool'" := ty_bool (in custom stlc_ty at level 0).
 
+Notation "x + y" := (tm_binop x tm_add y) (in custom stlc at level 2,
+                                              left associativity).
+Notation "x - y" := (tm_binop x tm_sub y) (in custom stlc at level 2,
+                                              left associativity).
+
+Notation "x * y" := (tm_binop x tm_mul y) (in custom stlc at level 1,
+                                              left associativity).
+Notation "x / y" := (tm_binop x tm_div y) (in custom stlc at level 1,
+                                              left associativity).
+Notation "x && y" := (tm_binop x tm_and y) (in custom stlc at level 2,
+                                              left associativity).
+Notation "x || y" := (tm_binop x tm_or y) (in custom stlc at level 2,
+                                              left associativity).
+Notation "x == y" := (tm_eq x y) (in custom stlc at level 1,
+                                     left associativity).
+Notation "! x " := (tm_not x) (in custom stlc at level 1,
+                                  left associativity).
+
+Notation "'if' x 'then' y 'else' z" :=
+  (tm_ifthenelse x y z) (in custom stlc at level 89,
+                    x custom stlc at level 99,
+                    y custom stlc at level 99,
+                    z custom stlc at level 99,
+                    left associativity).
+
+Notation "'let' x '=' t1 'in' t2" :=
+  (tm_let t1 (open_exp_wrt_exp t2 x)) (in custom stlc at level 0).
 
 Inductive multi {X : Type} (R : relation X) : relation X :=
   | multi_refl : forall (x : X), multi R x x
@@ -35,10 +67,37 @@ Inductive multi {X : Type} (R : relation X) : relation X :=
 
 Notation " t '-->*' t' " := (multi step t t') (at level 40).
 
-Inductive circuit_equiv(c: exp -> exp) (c': exp -> exp -> exp): Prop :=
-| Eq_Sound:
-    forall (v: exp) value v ->
-    exists (w: exp),
-      c x = const_field w ->
-      c' x w = const_true ->
-      circuit_equiv c c'.
+Definition div :=
+  <{ \X: Field, (100 / X) }>.
+
+Definition div_check :=
+  <{ \X: Field,
+         <{ \Y: Field,
+                X * Y == 100 }>
+   }>.
+
+Definition circuit_equiv(c: exp) (c': exp): Prop :=
+  forall (n: nat), exists (w: nat),
+   <{ c' n w }> -->* const_true ->
+   <{ c n }> -->* w.
+   
+Notation "a '~' b" := (circuit_equiv a b) (at level 50).
+Theorem div_gadget_proof: div ~ div_check.
+Proof.
+  unfold circuit_equiv, div, div_check.
+  induction 0.
+  - exists 0. intro H.
+    inversion H. subst.
+    inversion H0. subst.
+    
+  - inversion IHn.
+    
+    
+    eexists. intro.
+    split.
+    unfold div, div_check.
+    intro.
+    inversion H1.
+    
+    auto.
+    
